ITree_Hoare.thy
@@ -1,0 +1,64 @@
+section \<open> Hoare Logic \<close>
+
+theory ITree_Hoare
+  imports ITree_Relation
+begin
+
+definition hoare_triple :: "('s \<Rightarrow> bool) \<Rightarrow> ('e, 's) htree \<Rightarrow> ('s \<Rightarrow> bool) \<Rightarrow> bool" where
+"hoare_triple P S Q = (itree_rel S \<subseteq> spec \<top>\<^sub>S P Q)"
+
+syntax "_hoare" :: "logic \<Rightarrow> logic \<Rightarrow> logic \<Rightarrow> logic" ("\<^bold>{_\<^bold>} _ \<^bold>{_\<^bold>}")
+translations "_hoare P S Q" == "CONST hoare_triple (P)\<^sub>e S (Q)\<^sub>e"
+
+lemma hoare_alt_def: "\<^bold>{P\<^bold>} S \<^bold>{Q\<^bold>} \<longleftrightarrow> (\<forall> s s' es. P s \<and> S s \<midarrow>es\<leadsto> Ret s' \<longrightarrow> Q s')"
+  by (auto simp add: hoare_triple_def spec_def itree_rel_def retvals_def subset_iff)
+
+lemma hoareI: "\<lbrakk> \<And> s s' es. \<lbrakk> P s; S s \<midarrow>es\<leadsto> Ret s' \<rbrakk> \<Longrightarrow> Q s' \<rbrakk> \<Longrightarrow> \<^bold>{P\<^bold>} S \<^bold>{Q\<^bold>}"
+  by (auto simp add: hoare_alt_def)
+
+lemma hoare_while_partial:
+  assumes "\<^bold>{P \<and> B\<^bold>} S \<^bold>{P\<^bold>}"
+  shows "\<^bold>{P\<^bold>}while B do S od\<^bold>{\<not> B \<and> P\<^bold>}"
+proof (rule hoareI)
+  fix s s' tr
+  assume while: "P s" "while B do S od s \<midarrow>tr\<leadsto> \<cmark> s'"
+  show "\<not> B s' \<and> P s'"
+  proof (cases "B s")
+    case True
+    note B = this
+    obtain chn where chn: "itree_chain S s s' chn" "concat (map fst chn) = tr" "\<forall> i < length chn - 1. B (snd (chn ! i))" "\<not> B s'"
+      by (metis SEXP_def True iterate_term_chain while(2))
+    then interpret ichain: itree_chain S s s' chn by simp
+    have "\<forall> i < length chn. P (snd (chn ! i))"
+    proof (clarify)
+      fix i
+      assume i: "i < length chn"
+      thus "P (snd (chn ! i))"
+      proof (induct i)
+        case 0
+        hence "S s \<midarrow>fst (chn ! 0)\<leadsto> \<cmark> (snd (chn ! 0))"
+          by (metis gr_implies_not0 hd_conv_nth i ichain.chain_start length_0_conv)   
+        with assms while(1) B show ?case
+          by (auto simp add: hoare_alt_def)
+      next
+        case (Suc i)
+        hence "S (snd (chn ! i)) \<midarrow>fst (chn ! Suc i)\<leadsto> \<cmark> (snd (chn ! Suc i))"
+          by (metis Suc_eq_plus1 ichain.chain_iter less_diff_conv)
+        moreover have "B (snd (chn ! i))"
+          by (metis Suc.prems Suc_lessE chn(3) diff_Suc_1)
+        moreover have "P (snd (chn ! i))"
+          by (simp add: Suc.hyps Suc.prems Suc_lessD)
+        ultimately show ?case
+          using assms by (auto simp add: hoare_alt_def)
+      qed
+    qed
+    thus ?thesis
+      by (metis Suc_diff_1 chn(4) ichain.last_st ichain.length_chain last_conv_nth length_greater_0_conv lessI)
+  next
+    case False
+    then show ?thesis
+      using while(1) while(2) by force 
+  qed
+qed
+
+end
